src/vc0/preservation.lean
@@ -625,8 +625,8 @@ begin
     { exact is_field.cons (h_ih $ alist.mem_lookup_iff.2 m) } }
 end
 
-theorem default.ok {Γ : ast} {E ts v} (Γok : Γ.ok)
-  (h : default Γ ts v) : ok_type_or_sdef Γ E v ts :=
+theorem default.ok {Γ : ast} {ts v} (Γok : Γ.ok)
+  (h : default Γ ts v) (E) : ok_type_or_sdef Γ E v ts :=
 begin
   induction h,
   { exact ⟨_, vtype.of_ty.int, ok.int⟩ },
@@ -657,6 +657,16 @@ begin
       { cases h ⟨_, m⟩ },
       exact IH ((is_field_lookup tm).2 (alist.mem_lookup_iff.2 yf)) this } },
 end
+
+theorem default.ok' {Γ : ast} {t τ v} (ok : Γ.ok)
+  (h : default Γ (sum.inl t) v) (E)
+  (tτ : vtype.of_ty (exp.type.reg t) τ) : value.ok Γ E v τ :=
+let ⟨τ', h₁, h₂⟩ := h.ok ok E in vtype.of_ty_determ h₁ tτ ▸ h₂
+
+theorem ok.repeat {Γ E v τ} (h : value.ok Γ E v τ) :
+  ∀ {n}, value.ok Γ E (value.repeat v n) (vtype.arr' τ n)
+| 0     := value.ok.nil
+| (n+1) := value.ok.cons h ok.repeat
 
 end value
 
@@ -756,6 +766,11 @@ begin
     cases IH aok, exact a_3 _ _ _ _ _ hsd m tτ hf }
 end
 
+theorem ok.ref_opt {Γ E σ n τ}
+  (h : value.ok Γ E (value.ref n) (vtype.ref τ)) :
+  addr_opt.ok Γ E σ (addr.ref <$> n) τ :=
+by cases h; [trivial, exact addr.ok.ref h_a]
+
 end addr
 
 theorem assign.ok {Γ E Δ σ η x v t τ}
@@ -806,7 +821,13 @@ theorem value.step_binop.ok {Γ E op t₁ t₂ τ₁ τ₂ v₁ v₂ v}
   (tτ₂ : vtype.of_ty (exp.type.reg t₂) τ₂)
   (vok₁ : value.ok Γ E v₁ τ₁) (vok₂ : value.ok Γ E v₂ τ₁) :
   value.ok Γ E v τ₂ :=
-_
+begin
+  generalize_hyp e : sum.inl v = o at sok,
+  cases sok; cases opok; try {cases e}; cases tτ₁; cases tτ₂; try {constructor},
+  all_goals {
+    rcases (⟨_, e⟩ : ∃ x, sum.inl v = value.to_err x) with ⟨_|_, ⟨⟩⟩,
+    constructor }
+end
 
 theorem value.step_unop.ok {Γ E op t₁ t₂ τ₁ τ₂ v v'}
   (sok : value.step_unop op v v')
@@ -814,7 +835,7 @@ theorem value.step_unop.ok {Γ E op t₁ t₂ τ₁ τ₂ v v'}
   (tτ₁ : vtype.of_ty (exp.type.reg t₁) τ₁)
   (tτ₂ : vtype.of_ty (exp.type.reg t₂) τ₂)
   (vok₁ : value.ok Γ E v τ₁) : value.ok Γ E v' τ₂ :=
-_
+by cases sok; cases opok; cases tτ₁; cases tτ₂; constructor
 
 theorem stmt_list.ok.eq_none {Γ Δ δ ret}
   (Kok : stmt_list.ok Γ ret Δ δ []) : ret = none :=
@@ -836,11 +857,6 @@ begin
   { exact stmt_list.ok.weak (Kok_ih (finset.erase_subset_erase _ ss)) }
 end
 
--- theorem stmt_list.ok'.weak {Γ} {σ : vars_ty} {ret Δ K x τ h}
---   (Kok : stmt_list.ok' Γ (σ.erase x) ret Δ K) :
---   stmt_list.ok' Γ σ ret (Δ.cons x τ h) K :=
--- stmt_list.ok.weak (by simpa [stmt_list.ok'] using Kok)
-
 theorem stmt_list.ok.cons_inv {Γ E Δ σ η ret s K}
   (σok : vars_ty.ok Δ σ)
   (ηok : vars.ok Γ E η σ) : stmt_list.ok Γ ret Δ σ.keys (s :: K) →
@@ -859,15 +875,15 @@ begin
 end
 
 theorem step_deref.ok {Γ E σs Δ σ H S η ret a τ K s'}
-  (Cok : env.ok Γ ⟨E, σs, σ, Δ⟩ ⟨H, S, η⟩ ret)
+  (σok : vars_ty.ok Δ σ) (Eok : heap.ok Γ H E)
+  (ηok : vars.ok Γ E η σ) (Sok : stack.ok Γ E σs S ret)
   (aok : addr_opt.ok Γ E σ a τ)
   (Kok : cont.ok' Γ E σ Δ ret K τ)
   (h : step_deref ⟨H, S, η⟩ a K s') : state.ok Γ s' :=
 begin
   cases h,
   { apply state.ok.err },
-  { cases Cok with E σs σ H S η Δ _ σok Eok ηok Sok,
-    exact state.ok.ret ⟨σok, Eok, ηok, Sok⟩
+  { exact state.ok.ret ⟨σok, Eok, ηok, Sok⟩
       (h_a_1.ok σok Eok ηok aok) Kok }
 end
 
@@ -883,13 +899,22 @@ begin
   { apply state.ok.done }
 end
 
-theorem step_call.ok {Γ : ast} {E Δ f τ s vs τs η'}
-  (ok : Γ.ok)
-  (fd : Γ.get_body f τ Δ s)
-  (h : step_call vs η')
-  (vok : value.ok Γ E vs τs) :
-  ∃ σ', vars_ty.ok Δ σ' ∧ vars.ok Γ E η' σ' ∧ Δ.keys.to_finset ⊆ σ'.keys :=
-_
+theorem step_call.ok {Γ : ast} {Δ : ctx} {E vs τs η}
+  (τok : vtype.of_ty (exp.type.ls Δ.values) τs)
+  (sc : step_call Δ vs η) (vok : value.ok Γ E vs τs) :
+  ∃ σ, vars_ty.ok Δ σ ∧ vars.ok Γ E η σ ∧ Δ.keys.to_finset ⊆ σ.keys ∧ ∀ x ∈ η, x ∈ σ :=
+begin
+  induction sc with Δ x τ v vs η h a IH generalizing τs; cases τok; cases vok,
+  { exact ⟨∅, by rintro _ _ ⟨⟩, by rintro _ _ ⟨⟩, λ _, id, by rintro _ ⟨_, ⟨⟩⟩⟩ },
+  { rcases IH τok_a_1 vok_a_1 with ⟨σ, σok, ηok, ss, ησ⟩,
+    have ηok' := ηok.insert (mt (σok.mem ∘ ησ _) h) vok_a,
+    refine ⟨_, (σok.weak _).insert (mt σok.mem h) alist.lookup_cons_self τok_a,
+      ηok', _, λ y h, _⟩,
+    { rw [alist.cons_keys, list.cons_to_finset, finmap.keys_insert],
+      exact finset.insert_subset_insert _ ss },
+    { rw [← finmap.mem_keys, finmap.keys_insert, finset.mem_insert, finmap.mem_keys] at h ⊢,
+      exact h.imp_right (ησ _) } }
+end
 
 theorem step_alloc.ok {Γ E σs Δ σ H S ret η τ v K s}
   (σok : vars_ty.ok Δ σ) (Eok : heap.ok Γ H E)
@@ -911,7 +936,6 @@ theorem preservation {Γ : ast} (ok : Γ.ok)
   {s'} (H : step Γ s o s') : state.ok Γ s' :=
 begin
   cases H,
-  /-
   case c0.step.decl : H S η v τ τ' s K H₁ {
     rcases sok with ⟨_, _, _, _, _, τ, _, _, _, t,
       ⟨E, σs, σ, H, η, S, Δ, _, σok, Eok, ηok, Sok⟩,
@@ -1012,7 +1036,7 @@ begin
     rcases sok with _|_|⟨E, σs, σ, H, η, S, Δ, ret, τ, α, v, K,
       ⟨E, σs, σ, H, η, S, Δ, _, σok, Eok, ηok, Sok⟩,
       aok, Kok⟩, cases Kok, cases Kok_a with _ opok,
-    exact step_deref.ok ⟨σok, Eok, ηok, Sok⟩ aok
+    exact step_deref.ok σok Eok ηok Sok aok
       (cont.ok.binop₁ opok Kok_a_1 Kok_a_1 Kok_a_2 Kok_a_3 $
        cont.ok.asgn₂ aok Kok_a_4) h },
   case c0.step.eval₁ : C e K {
@@ -1190,8 +1214,8 @@ begin
       ⟨E, σs, σ, H, η, S, Δ, _, σok, Eok, ηok, Sok⟩,
       vok, Kok⟩, cases Kok,
     cases ok.fdef_uniq _ _ _ bok.get_fdef Kok_a,
-    rcases step_call.ok ok bok sc vok with ⟨σ', σok', ηok', ss⟩,
-    rcases get_body_ok' ok bok with ⟨sok, r, δ, si⟩,
+    rcases sc.ok Kok_a_2 vok with ⟨σ', σok', ηok', ss, _⟩,
+    rcases get_body_ok' ok.ind bok with ⟨sok, r, δ, si⟩,
     rcases si.mono ss with ⟨δ', ss', si'⟩,
     exact state.ok.stmt _ ⟨σok', Eok, ηok', Sok.cons σok ηok Kok_a_3⟩
       Kok_a_1 sok si' (r.imp_right stmt_list.ok.nil) },
@@ -1222,15 +1246,86 @@ begin
       eu, ⟨t, eok, tτ⟩, Kok⟩, cases eok,
     exact state.ok.exp ⟨σok, Eok, ηok, Sok⟩ eu ⟨_, eok_a, vtype.of_ty.struct⟩
       (cont.ok.addr_field eok_a_1 eok_a_2 tτ $ cont.ok.deref Kok) },
-  -/
+  case c0.step.deref' : C a K sd {
+    rcases sok with _|_|⟨E, σs, σ, H, η, S, Δ, ret, τ, α, v, K,
+      ⟨E, σs, σ, H, η, S, Δ, _, σok, Eok, ηok, Sok⟩,
+      aok, Kok⟩, cases Kok,
+    exact sd.ok σok Eok ηok Sok aok Kok_a },
   case c0.step.alloc_ref : C τ τ' v K ττ' v0 sa {
     rcases sok with _|⟨E, σs, σ, H, η, S, Δ, ret, τ, α, v, K,
       ⟨E, σs, σ, H, η, S, Δ, _, σok, Eok, ηok, Sok⟩,
       eu, ⟨t, eok, tτ⟩, Kok⟩, cases eok,
-    refine sa.ok σok Eok ηok Sok _ _, },
-
+    cases ast.eval_ty.determ ok.ind ττ' eok_a, cases tτ,
+    refine sa.ok σok Eok ηok Sok (v0.ok' ok _ tτ_a) Kok },
+  case c0.step.alloc_arr₁ : C τ τ' e K ττ' {
+    rcases sok with _|⟨E, σs, σ, H, η, S, Δ, ret, τ, α, v, K,
+      ⟨E, σs, σ, H, η, S, Δ, _, σok, Eok, ηok, Sok⟩,
+      eu, ⟨t, eok, tτ⟩, Kok⟩, cases eok,
+    cases ast.eval_ty.determ ok.ind ττ' eok_a, cases tτ,
+    exact state.ok.exp ⟨σok, Eok, ηok, Sok⟩ eu ⟨_, eok_a_2, vtype.of_ty.int⟩
+      (cont.ok.alloc_arr tτ Kok) },
+  case c0.step.alloc_arr₂ : C τ v K i n e v0 sa {
+    rcases sok with _|_|⟨E, σs, σ, H, η, S, Δ, ret, τ, α, v, K,
+      ⟨E, σs, σ, H, η, S, Δ, _, σok, Eok, ηok, Sok⟩,
+      vok, Kok⟩, cases Kok, cases Kok_a,
+    exact sa.ok σok Eok ηok Sok (v0.ok' ok _ Kok_a_a).repeat.arr Kok_a_1 },
+  case c0.step.alloc_arr_err : C τ i K i0 { apply state.ok.err },
+  case c0.step.addr_var : C v K {
+    rcases sok with _|⟨E, σs, σ, H, η, S, Δ, ret, τ, α, v, K,
+      ⟨E, σs, σ, H, η, S, Δ, _, σok, Eok, ηok, Sok⟩,
+      eu, ⟨t, eok, tτ⟩, Kok⟩, cases eok,
+    rcases finmap.exists_mem_lookup_iff.2
+      (finmap.mem_keys.1 $ finset.singleton_subset.1 eu) with ⟨τ', vτ'⟩,
+    cases vtype.of_ty_determ (σok.ok_of_mem vτ' eok_a) tτ,
+    exact state.ok.ret ⟨σok, Eok, ηok, Sok⟩ (addr.ok.var vτ') Kok },
+  case c0.step.addr_deref₁ : C e K {
+    rcases sok with _|⟨E, σs, σ, H, η, S, Δ, ret, τ, α, v, K,
+      ⟨E, σs, σ, H, η, S, Δ, _, σok, Eok, ηok, Sok⟩,
+      eu, ⟨t, eok, tτ⟩, Kok⟩, cases eok,
+    exact state.ok.exp ⟨σok, Eok, ηok, Sok⟩ eu ⟨_, eok_a, tτ.ref⟩
+      (cont.ok.addr_deref Kok) },
+  case c0.step.addr_deref₂ : C v K {
+    rcases sok with _|_|⟨E, σs, σ, H, η, S, Δ, ret, τ, α, v, K,
+      ⟨E, σs, σ, H, η, S, Δ, _, σok, Eok, ηok, Sok⟩,
+      vok, Kok⟩, cases Kok,
+    refine state.ok.ret ⟨σok, Eok, ηok, Sok⟩ (addr.ok.ref_opt vok) Kok_a },
+  case c0.step.addr_index₁ : C e n K {
+    rcases sok with _|⟨E, σs, σ, H, η, S, Δ, ret, τ, α, v, K,
+      ⟨E, σs, σ, H, η, S, Δ, _, σok, Eok, ηok, Sok⟩,
+      eu, ⟨t, eok, tτ⟩, Kok⟩, cases eok,
+    have eu₁ := finset.subset.trans (finset.subset_union_left _ _) eu,
+    have eu₂ := finset.subset.trans (finset.subset_union_right _ _) eu,
+    exact state.ok.exp ⟨σok, Eok, ηok, Sok⟩ eu₁ ⟨_, eok_a, tτ.arr⟩
+      (cont.ok.addr_index₁ eok_a_1 eu₂ Kok) },
+  case c0.step.addr_index₂ : C a n K {
+    rcases sok with _|_|⟨E, σs, σ, H, η, S, Δ, ret, τ, α, v, K,
+      ⟨E, σs, σ, H, η, S, Δ, _, σok, Eok, ηok, Sok⟩,
+      vok, Kok⟩, cases Kok,
+    refine state.ok.exp ⟨σok, Eok, ηok, Sok⟩ Kok_a_1 ⟨_, Kok_a, vtype.of_ty.int⟩
+      (cont.ok.addr_index₂ (addr.ok.ref_opt vok) Kok_a_2) },
+  case c0.step.addr_index₃ : C a n K i j len e lt {
+    rcases sok with _|_|⟨E, σs, σ, H, η, S, Δ, ret, τ, α, v, K,
+      ⟨E, σs, σ, H, η, S, Δ, _, σok, Eok, ηok, Sok⟩,
+      _, Kok⟩, cases Kok,
+    cases len with _ _ v len,
+    exact state.ok.ret ⟨σok, Eok, ηok, Sok⟩ (addr.ok.nth Kok_a_1) Kok_a_2 },
+  case c0.step.addr_index_err₁ : C i K { apply state.ok.err },
+  case c0.step.addr_index_err₂ : C a n i K { apply state.ok.err },
+  case c0.step.addr_field₁ : C e f K {
+    rcases sok with _|⟨E, σs, σ, H, η, S, Δ, ret, τ, α, v, K,
+      ⟨E, σs, σ, H, η, S, Δ, _, σok, Eok, ηok, Sok⟩,
+      eu, ⟨t, eok, tτ⟩, Kok⟩, cases eok,
+    exact state.ok.exp ⟨σok, Eok, ηok, Sok⟩ eu ⟨_, eok_a, vtype.of_ty.struct⟩
+      (cont.ok.addr_field eok_a_1 eok_a_2 tτ Kok) },
+  case c0.step.addr_field₂ : C a f K {
+    rcases sok with _|_|⟨E, σs, σ, H, η, S, Δ, ret, τ, α, v, K,
+      ⟨E, σs, σ, H, η, S, Δ, _, σok, Eok, ηok, Sok⟩,
+      aok, Kok⟩, cases Kok,
+    exact state.ok.ret ⟨σok, Eok, ηok, Sok⟩
+      (addr.ok.field Kok_a Kok_a_1 Kok_a_2 aok) Kok_a_3 },
+  case c0.step.addr_field_err : C f K { apply state.ok.err }
 end
-#print ast.stmt.init.mono
+
 theorem progress {Γ : ast} (ok : Γ.ok)
   {s} (h₁ : state.ok Γ s) : s.final ∨ ∃ o s', step Γ s o s' :=
 sorry
